Java/src/Java/Logic/SpecLogic.v
@@ -9,7 +9,7 @@ Local Existing Instance ILPre_Ops.
 Local Existing Instance ILPre_ILogic.
 *)
 
-Definition spec := ILPreFrm Prog_wf_sub (ILPreFrm ge Prop).
+Definition spec := ILPreFrm Prog_sub (ILPreFrm ge Prop).
 
 (*
 Global Instance ILLOperatorsSpec : ILLOperators spec := _.
@@ -19,12 +19,12 @@ Global Instance ILSpec : ILLater spec := _.
 
 Local Transparent ILPre_Ops.
 Require Import Compare_dec.
-Definition mk_spec (f: Prog_wf -> nat -> Prop)
+Definition mk_spec (f: Program -> nat -> Prop)
   (Hnat: forall k P, f P (S k) -> f P k)
-  (HSPred: forall k P P', Prog_wf_sub P P' -> f P k -> f P' k) : spec.
+  (HSPred: forall k P P', Prog_sub P P' -> f P k -> f P' k) : spec.
   refine (mkILPreFrm (fun k => mkILPreFrm (f k) _) _).
 Proof.
-  assert (forall k P P', Prog_wf_sub P P' -> f P k -> f P' k) as HProg.
+  assert (forall k P P', Prog_sub P P' -> f P k -> f P' k) as HProg.
   intros k P P' HPP' S'. eapply HSPred; eassumption. 
   intros p p' Hp'' n S'; simpl in *. eapply HProg; eassumption.
   Grab Existential Variables.
@@ -36,7 +36,7 @@ Proof.
 Defined.
 
 Program Definition prog_spec (X : Program -> Prop) : spec :=
-  mk_spec (fun (P : Prog_wf) _ => forall (Q : Prog_wf) , Prog_sub P Q -> X Q) _ _.
+  mk_spec (fun (P : Program) _ => forall (Q : Program) , Prog_sub P Q -> X Q /\ valid_program Q = true) _ _.
 Next Obligation.
   intros; apply H0; etransitivity; eassumption.
 Qed.
@@ -57,5 +57,5 @@ Lemma prog_eq_to_prop P (f : Program -> Prop) (H : f P) : prog_eq P |-- [prog] f
 Proof.
   intros Q n HQ R HQR.
   specialize (HQ _ HQR).
-  simpl in *. subst. apply H.
+  simpl in *. subst. intuition congruence.
 Qed.
